More proof setup

compiler/wasm/stack_to_wasmProofScript.sml
@@ -3,13 +3,201 @@
 *)
 Theory stack_to_wasmProof
 Ancestors
-  wasmLang stackLang words arithmetic list rich_list sptree mlstring
-  wasmSem stackSem
+  wasmLang words arithmetic list rich_list sptree mlstring
+  wasmSem stackSem stackLang
 Libs
-  wordsLib
+  wordsLib helperLib
 
-Theorem placeholder:
-  T
+(* definitions used in the correctness statement *)
+
+val s = “s:('a,'c,'ffi) stackSem$state”
+val t = “t:wasmSem$state”
+
+Definition empty_buffer_def:
+  empty_buffer b ⇔
+    b.position = 0w ∧
+    b.buffer = [] ∧
+    b.space_left = 0
+End
+
+Definition state_rel_def:
+  state_rel ^s ^t ⇔
+    ¬ s.use_stack ∧ ¬ s.use_store ∧ ¬ s.use_alloc ∧ ¬ s.be ∧
+    empty_buffer s.code_buffer ∧ empty_buffer s.data_buffer
+End
+
+(* set up for one theorem per case *)
+
+val goal_tm =
+  “λ(p,^s). ∀res s1 t.
+     evaluate (p,s) = (res,s1) ∧
+     state_rel s t ∧
+     res ≠ SOME Error ⇒
+     ∃ck t1 res1.
+       exec (compile p) (t with clock := t.clock + ck) = (res1,t1) ∧
+       state_rel s1 t1”
+
+local
+  val ind_thm = stackSemTheory.evaluate_ind |> ISPEC goal_tm
+    |> CONV_RULE (DEPTH_CONV PairRules.PBETA_CONV)
+  val ind_goals = ind_thm |> concl |> dest_imp |> fst |> helperLib.list_dest dest_conj
+in
+  fun get_goal s =
+    first (can (find_term (can (match_term (Term [QUOTE ("stackLang$"^s)]))))) ind_goals
+  fun compile_correct_tm () = ind_thm |> concl |> rand
+  fun the_ind_thm () = ind_thm
+end
+
+(* a proof for each case *)
+
+Theorem compile_Skip:
+  ^(get_goal "Skip")
 Proof
-  fs []
+  cheat
 QED
+
+Theorem compile_Inst:
+  ^(get_goal "Inst")
+Proof
+  cheat
+QED
+
+Theorem compile_Call:
+  ^(get_goal "Call")
+Proof
+  cheat
+QED
+
+Theorem compile_Seq:
+  ^(get_goal "Seq")
+Proof
+  cheat
+QED
+
+Theorem compile_If:
+  ^(get_goal "If")
+Proof
+  cheat
+QED
+
+Theorem compile_While:
+  ^(get_goal "While")
+Proof
+  cheat
+QED
+
+Theorem compile_JumpLower:
+  ^(get_goal "JumpLower")
+Proof
+  cheat
+QED
+
+Theorem compile_Alloc:
+  ^(get_goal "Alloc")
+Proof
+  cheat
+QED
+
+Theorem compile_StoreConsts:
+  ^(get_goal "StoreConsts")
+Proof
+  cheat
+QED
+
+Theorem compile_Raise:
+  ^(get_goal "Raise")
+Proof
+  cheat
+QED
+
+Theorem compile_Return:
+  ^(get_goal "Return")
+Proof
+  cheat
+QED
+
+Theorem compile_FFI:
+  ^(get_goal "FFI")
+Proof
+  cheat
+QED
+
+Theorem compile_Tick:
+  ^(get_goal "Tick")
+Proof
+  cheat
+QED
+
+Theorem compile_LocValue:
+  ^(get_goal "LocValue")
+Proof
+  cheat
+QED
+
+Theorem compile_Install:
+  ^(get_goal "Install")
+Proof
+  cheat
+QED
+
+Theorem compile_ShMemOp:
+  ^(get_goal "ShMemOp")
+Proof
+  cheat
+QED
+
+Theorem compile_RawCall:
+  ^(get_goal "RawCall")
+Proof
+  cheat
+QED
+
+Theorem compile_BitmapLoad:
+  ^(get_goal "BitmapLoad")
+Proof
+  cheat
+QED
+
+Theorem compile_Halt:
+  ^(get_goal "Halt")
+Proof
+  cheat
+QED
+
+Theorem compile_CodeBufferWrite:
+  ^(get_goal "CodeBufferWrite")
+Proof
+  rw [evaluate_def,wordSemTheory.buffer_write_def]
+  \\ fs [state_rel_def,empty_buffer_def,AllCaseEqs()]
+QED
+
+Theorem compile_DataBufferWrite:
+  ^(get_goal "DataBufferWrite")
+Proof
+  rw [evaluate_def,wordSemTheory.buffer_write_def]
+  \\ fs [state_rel_def,empty_buffer_def,AllCaseEqs()]
+QED
+
+(* combining all the cases to prove main simulation theorem *)
+
+Theorem compile_correct:
+  ^(compile_correct_tm())
+Proof
+  match_mp_tac (the_ind_thm())
+  \\ EVERY (map strip_assume_tac [compile_Skip, compile_Inst,
+       compile_Call, compile_Seq, compile_If, compile_While,
+       compile_JumpLower, compile_Alloc, compile_StoreConsts,
+       compile_Raise, compile_Return, compile_FFI, compile_Tick,
+       compile_LocValue, compile_Install, compile_ShMemOp,
+       compile_CodeBufferWrite, compile_DataBufferWrite,
+       compile_RawCall, compile_BitmapLoad, compile_Halt])
+  \\ asm_rewrite_tac []
+  \\ rpt $ pop_assum kall_tac
+  \\ rw [evaluate_def,state_rel_def]
+QED
+
+(*
+  TypeBase.constructors_of “:'a stackLang$prog”
+  |> map term_to_string
+  |> map (fn s => print ("\n    compile_" ^ s ^ ","))
+*)
